some WIP I don't remember what

Infer.v
@@ -60,7 +60,7 @@ intro. unfold unifies_all in H.
 apply (wildcard' s). unfold unifies_all. intros. apply H. right. assumption.
 Qed.
 
-Require Import FMapInterface Equalities.
+Require Import FMapFacts Equalities.
 
 Instance string_Equivalence : Equivalence eq (A := string) := {}.
 
@@ -73,6 +73,7 @@ End string_EQ.
 
 Module old_string_EQ := Backport_DT string_EQ.
 Module Infer (Map : WSfun old_string_EQ).
+Module MF := WFacts_fun old_string_EQ Map.
 
 Definition unify_sets sets : list (Tipe * Tipe) :=
 let set_to_pairs set :=
@@ -102,12 +103,20 @@ end.
 Definition Env := Map.t Tipe.
 Definition values {A} (m : Map.t A) : list A := map snd (Map.elements m).
 Definition singleton a (x : Tipe) := Map.add a x (Map.empty _).
-Lemma singleton_values : forall n a b, In b (values (singleton n a)) -> a = b.
-intros. pose proof Map.elements_2. specialize H0 with Tipe (singleton n a) n b.
-destruct (eq_dec a b). assumption.
-pose proof Map.add_3. Admitted.
+Lemma singleton_MapsTo : forall k v, Map.MapsTo k v (singleton k v).
+intros. compute. apply Map.add_1. reflexivity.
+Qed.
+Lemma singleton_MapsTo_one_thing : forall a b c d, Map.MapsTo a b (singleton c d) -> a = c /\ b = d.
+intros.
+destruct (string_dec a c); destruct (eq_dec b d).
+  auto.
+  assert (Map.MapsTo a d (singleton c d)). apply Map.add_1. easy.
+    apply Map.find_1 in H. apply Map.find_1 in H0. rewrite H in H0.
+    injection H0. auto.
+  all: apply Map.add_3 in H; [ apply Map.empty_1 in H; contradiction | auto ].
+Qed.
 
-Lemma MapsTo_in_values {A} : forall v m k, Map.MapsTo k v m -> In v (values (A := A) m).
+Lemma MapsTo_in_values {A} : forall k v m, Map.MapsTo k v m -> In v (values (A := A) m).
 intros. unfold values. apply Map.elements_1 in H.
 Admitted.
 
@@ -141,10 +150,40 @@ Notation "a '-> b" := (TApp (TApp (TConst "->") a) b) (at level 59, right associ
 
 Definition vars_below n t := forall v, Contains (TVar v) t -> v < n.
 
-Inductive typing :=
-  mk_typing : forall t e (n : nat),
+Definition typing : Type := Tipe * Env.
+
+Inductive well_typed : expression -> typing -> Prop :=
+| wt_Var : forall name env t,
+    Map.find name env = Some t -> well_typed (Var name) (t, env)
+| wt_Lambda : forall name body env argt returnt,
+    well_typed body (returnt, Map.add name argt env) -> well_typed (Lambda name body) (argt '-> returnt, env)
+| wt_Call : forall f x argt returnt env,
+    well_typed f (argt '-> returnt, env) -> well_typed x (argt, env) -> well_typed (Call f x) (returnt, env).
+
+Lemma equal_env_wt : forall e t env env2,
+  well_typed e (t, env) -> Map.Equal env env2 -> well_typed e (t, env2).
+induction e.
+  intros. dependent destruction H. apply wt_Var. rewrite H0 in H. assumption.
+  intros. dependent destruction H. apply wt_Lambda.
+    apply (IHe returnt (Map.add n argt env)). assumption. compute. intros.
+    destruct (string_dec y n).
+      repeat rewrite MF.add_eq_o. easy. easy. easy.
+      repeat rewrite MF.add_neq_o. auto. auto. auto.
+  intros. dependent destruction H. apply (wt_Call e1 e2 argt).
+    apply (IHe1 (argt '-> t) env). assumption. assumption.
+    apply (IHe2 argt env). assumption. assumption.
+Qed.
+
+Definition most_general_type e (t : typing) := forall t2, well_typed e t2
+  -> exists s, (apply s (fst t) = fst t2
+  /\ forall x a, Map.find x (snd t) = Some a -> Map.find x (snd t2) = Some (apply s a)).
+
+Definition typing_with_varcount : Type := typing * nat.
+
+Inductive typing_nvars : typing_with_varcount -> Prop :=
+  mk_typing_nvars : forall t e (n : nat),
   vars_below n t /\ (forall t2, In t2 (values e) -> vars_below n t2)
-  -> typing.
+  -> typing_nvars (t, e, n).
 
 Fixpoint add_to_tvars x t :=
 match t with
@@ -153,54 +192,86 @@ match t with
 | TApp a b => TApp (add_to_tvars x a) (add_to_tvars x b)
 end.
 
-Program Fixpoint infer (e : expression) {measure (esize e)} : option typing :=
+Program Fixpoint infer (e : expression) {measure (esize e)} :
+  { t | well_typed e (fst t) /\ most_general_type e (fst t) /\ typing_nvars t} + { forall t, ~ well_typed e t } :=
 match e with
-| Var a => Some (mk_typing (TVar 0) (singleton a (TVar 0)) 1 _)
+| Var a => inleft (TVar 0, (singleton a (TVar 0)), 1)
 | Lambda x b =>
   match infer b with
-  | Some (mk_typing t env n _) =>
+  | inleft (exist _ (t, env, n) _) =>
     match Map.find x env with
-    | Some argt => Some (mk_typing (argt '-> t) (Map.remove x env) n _)
-    | None => Some (mk_typing (TVar n '-> t) env (S n) _)
+    | Some argt => inleft (argt '-> t, Map.remove x env, n)
+    | None => inleft (TVar n '-> t, env, (S n))
     end
-  | None => None
+  | inright _ => inright _
   end
 | Call f x =>
-  match infer f, infer x with
-  | Some (mk_typing f_t f_env f_n _), Some (mk_typing x_t_ x_env_ x_n _) =>
-    let x_t := add_to_tvars f_n x_t_ in
-    let x_env := Map.map (add_to_tvars f_n) x_env_ in
-    let (env, pairs) := merge_envs [f_env; x_env] in
-    let return_value := TVar (f_n + x_n) in
-    match unify_many ((f_t, x_t '-> return_value) :: pairs) with
-    | inleft _ s => Some (mk_typing (apply s return_value) (Map.map (apply s) env) (S (f_n + x_n)) _)
-    | _ => None
+  match infer f with
+  | inleft (exist _ (f_t, f_env, f_n) _) =>
+    match infer x with
+    | inleft (exist _ (x_t_, x_env_, x_n_) _) =>
+      let x_t := add_to_tvars f_n x_t_ in
+      let x_env := Map.map (add_to_tvars f_n) x_env_ in
+      let x_n := x_n_ + f_n in
+      let (env, pairs) := merge_envs [f_env; x_env] in
+      let return_value := TVar x_n in
+      match unify_many ((f_t, x_t '-> return_value) :: pairs) with
+      | inleft _ s => inleft (apply s return_value, Map.map (apply s) env, S x_n)
+      | _ => inright _
+      end
+    | _ => inright _
     end
-  | _, _ => None
+  | _ => inright _
   end
 end.
 
-Next Obligation.
-split; [ | intros; apply singleton_values in H; destruct H ].
-all: compute; intros; dependent destruction H; easy.
+Next Obligation. split.
+apply wt_Var. apply Map.find_1. apply singleton_MapsTo.
+
+split.
+unfold most_general_type. intros. dependent destruction H. simpl.
+exists (sole_sub 0 t). split. easy.
+intros. apply Map.find_2 in H0. apply singleton_MapsTo_one_thing in H0. destruct H0. destruct H0. rewrite H1.
+easy.
+
+apply mk_typing_nvars.
+split; [ | intros; apply values_in_map in H; destruct H;
+  apply singleton_MapsTo_one_thing in H; destruct H; rewrite H0 ].
+compute; intros; dependent destruction H; easy.
+compute. intros. dependent destruction H1. easy.
 Qed.
 
-Next Obligation.
-apply eq_sym in Heq_anonymous. apply Map.find_2 in Heq_anonymous. apply MapsTo_in_values in Heq_anonymous.
-apply v0 in Heq_anonymous.
+Next Obligation. split.
+apply wt_Lambda. apply (equal_env_wt b t env). assumption.
+unfold Map.Equal. intro. destruct (string_dec x y).
+  rewrite MF.add_eq_o. congruence. assumption.
+  rewrite MF.add_neq_o. rewrite MF.remove_neq_o. reflexivity. assumption. assumption.
+
 split.
+unfold most_general_type. intros.
+destruct t2. simpl. dependent destruction H. apply m in H. destruct H. simpl in H.
+exists x0. rewrite H.
+
+apply mk_typing_nvars. dependent destruction t0. destruct a. split.
 unfold vars_below. intros. dependent destruction H. dependent destruction H.
-  dependent destruction H. auto. auto.
+  dependent destruction H. apply v0 in H. assumption. apply (MapsTo_in_values x argt env). apply MF.find_mapsto_iff. auto. auto.
 intros. apply v0. apply values_in_map in H. destruct H. apply Map.remove_3 in H. apply MapsTo_in_values in H.
 assumption.
 Qed.
 
-Next Obligation.
-split.
+Next Obligation. split.
+apply (wt_Lambda (S n)). give_up.
+(* liian helppo todistaa. hyväksyisi mitä vaan argumentin tyypiksi *)
+
+dependent destruction t0. destruct a. split. split.
   unfold vars_below. intros. dependent destruction H. dependent destruction H. dependent destruction H.
     dependent destruction H. omega.
     apply v in H. auto.
   intros. apply v0 in H. unfold vars_below. intros. unfold vars_below in H. apply H in H0. omega.
+Admitted.
+
+Next Obligation.
+intro. dependent destruction H. apply wildcard' in H. easy.
 Qed.
 
 Next Obligation.
